pulse/share/steel/examples/pulse/lib/pledge/Pulse.Lib.InvList.fsti
@@ -2,7 +2,8 @@ module Pulse.Lib.InvList
 
 open Pulse.Lib.Pervasives
 
-let invlist0 = list (p:vprop & inv p)
+let invlist_elem = p:vprop & inv p
+let invlist0 = list invlist_elem
 
 let rec invlist_names (is : invlist0) : inames =
   match is with
@@ -16,6 +17,9 @@ let rec invlist_nodups (is : invlist0) : prop =
 
 let invlist =
   i:invlist0{invlist_nodups i}
+
+let add_one (h : invlist_elem) (t : invlist{not (mem_inv (invlist_names t) (dsnd h))}) : invlist =
+  h :: t
 
 let rec invlist_v (is : invlist) : vprop =
   match is with
@@ -36,3 +40,12 @@ val with_invlist (#a:Type0) (#pre : vprop) (#post : a -> vprop)
   (is : invlist)
   (f : unit -> stt_unobservable a emp_inames (invlist_v is ** pre) (fun v -> invlist_v is ** post v))
   : stt_unobservable a (invlist_names is) pre (fun v -> post v)
+
+(* A helper for a ghost-unit function. *)
+val with_invlist_ghost (#pre : vprop) (#post : vprop)
+  (is : invlist)
+  (f : unit -> stt_ghost unit emp_inames (invlist_v is ** pre) (fun _ -> invlist_v is ** post))
+  : stt_unobservable unit (invlist_names is) pre (fun _ -> post)
+
+let invlist_sub (is1 is2 : invlist) : prop =
+  inames_subset (invlist_names is1) (invlist_names is2)
